cleaning up

src/Bedrock/End2End/X25519/MontgomeryLadder.v
@@ -16,59 +16,34 @@ Require Import Crypto.Bedrock.Group.ScalarMult.LadderStep.
 Require Import Crypto.Bedrock.Group.ScalarMult.CSwap.
 Require Import Crypto.Bedrock.Group.ScalarMult.MontgomeryLadder.
 Require Import Crypto.Bedrock.End2End.X25519.Field25519.
-Require Import Crypto.Bedrock.Specs.Field.
 Local Open Scope string_scope.
-Local Open Scope Z_scope.
 Import ListNotations.
 
 Local Instance frep25519 : Field.FieldRepresentation(field_parameters:=field_parameters) := field_representation n Field25519.s c.
+Derive ladderstep SuchThat (ladderstep = ladderstep_body) As ladderstep_defn.
+Proof. vm_compute. subst; exact eq_refl. Qed.
+
+Derive montladder SuchThat (montladder = montladder_body (Z.to_nat (Z.log2 Curve25519.order)))
+       As montladder_defn.
+Proof. vm_compute. subst; exact eq_refl. Qed.
 
 Require Import bedrock2.NotationsCustomEntry.
 
-Definition square_and_add := func! (o, x, y) {
-  fe25519_square(o, x);
-  fe25519_add(o, o, y)
+Definition x25519 := func! (out, sk, pk) {
+  stackalloc 40 as U;
+  fe25519_from_bytes(U, pk);
+  stackalloc 40 as OUT;
+  montladder(OUT, sk, U);
+  fe25519_to_bytes(out, OUT)
 }.
 
-Definition mul_and_add := func! (o, x, y) {
-  fe25519_mul(o, x, x);
-  fe25519_add(o, o, y)
+Definition x25519_base := func! (out, sk) {
+  stackalloc 40 as U;
+  fe25519_from_word(U, $9);
+  stackalloc 40 as OUT;
+  montladder(OUT, sk, U);
+  fe25519_to_bytes(out, OUT)
 }.
-
-(* Better way to represent points in Bedrock2? *)
-Definition add_precomputed := func! (ox, oy, oz, ot, X1, Y1, Z1, T1, ypx2, ymx2, xy2d2) {
-  stackalloc 40 as YpX1;
-  fe25519_add(YpX1, Y1, X1);
-  stackalloc 40 as YmX1;
-  fe25519_sub(YmX1, Y1, X1);
-  stackalloc 40 as A;
-  fe25519_mul(A, YpX1, ypx2);
-  stackalloc 40 as B;
-  fe25519_mul(B, YmX1, ymx2);
-  stackalloc 40 as C;
-  fe25519_mul(C, xy2d2, T1);
-  stackalloc 40 as D;
-  fe25519_add(D, Z1, Z1);
-  fe25519_sub(ox, A, B);
-  fe25519_add(oy, A, B);
-  fe25519_add(oz, D, C);
-  fe25519_sub(ot, D, C);
-  fe25519_mul(ox, ox, ot);
-  fe25519_mul(oy, oy, oz);
-  fe25519_mul(oz, ot, oz);
-  fe25519_mul(ot, ox, oy)
-}.
-
-Require Import bedrock2.FE310CSemantics bedrock2.Semantics .
-Require Import bedrock2.WeakestPrecondition bedrock2.ProgramLogic.
-Require Import coqutil.Word.Interface coqutil.Word.Bitwidth.
-Require Import coqutil.Map.Interface bedrock2.Map.SeparationLogic.
-Require Import bedrock2.Array bedrock2.Scalars.
-Require Import bedrock2.ZnWords.
-Require Import coqutil.Tactics.Tactics.
-
-Section WithParameters.
-  Check _: FieldRepresentation.
 
 Import LittleEndianList.
 Local Coercion F.to_Z : F >-> Z.
@@ -78,161 +53,177 @@ Require Import coqutil.Map.OfListWord Coq.Init.Byte coqutil.Byte.
 Import ProgramLogic.Coercions.
 Local Notation "m =* P" := ((P%sep) m) (at level 70, only parsing) (* experiment*).
 Local Notation "xs $@ a" := (Array.array ptsto (word.of_Z 1) a xs) (at level 10, format "xs $@ a").
+Definition x25519_gallina := montladder_gallina (Field.M_pos(FieldParameters:=field_parameters)) Field.a24 (Z.to_nat (Z.log2 (Z.pos order))).
+Global Instance spec_of_x25519 : spec_of "x25519" :=
+  fnspec! "x25519" out sk pk / (o s p : list Byte.byte) (R : _ -> Prop),
+  { requires t m := m =* s$@sk * p$@pk * o$@out * R /\
+      length s = 32%nat /\ length p = 32%nat /\ length o = 32%nat /\ byte.unsigned (nth 31 p x00) <= 0x7f;
+    ensures t' m := t=t' /\ m=* s$@sk ⋆ p$@pk ⋆ R ⋆
+      (le_split 32 (x25519_gallina (le_combine s) (Field.feval_bytes p)))$@out }.
 
-Local Notation FElem := (FElem(FieldRepresentation:=frep25519)).
-Local Notation bounded_by := (bounded_by(FieldRepresentation:=frep25519)).
-Local Notation word := (Naive.word 32).
-Local Notation felem := (felem(FieldRepresentation:=frep25519)).
-
-Global Instance spec_of_square_and_add : spec_of "square_and_add" :=
-  fnspec! "square_and_add" (out xk yk: word) / (o x y : felem) (R : _ -> Prop),
-  { requires t m :=
-      bounded_by loose_bounds x /\
-      bounded_by tight_bounds y /\
-      m =* (FElem xk x) * (FElem yk y) * (FElem out o) * R;
-    ensures t' m' :=
-      t=t' /\
-      exists o', feval o' = F.add (F.pow (feval x) 2) (feval y)
-        /\ bounded_by loose_bounds o'
-        /\ m' =* (FElem xk x) * (FElem yk y) * (FElem out o') * R }.
-
-Global Instance spec_of_mul_and_add : spec_of "mul_and_add" :=
-  fnspec! "mul_and_add" (out xk yk: word) / (o x y : felem) (R : _ -> Prop),
-  { requires t m :=
-      bounded_by loose_bounds x /\
-      bounded_by tight_bounds y /\
-      m =* (FElem xk x) * (FElem yk y) * (FElem out o) * R;
-    ensures t' m' :=
-      t=t' /\
-      exists o', feval o' = F.add (F.mul (feval x) (feval x)) (feval y)
-        /\ bounded_by loose_bounds o'
-        /\ m' =* (FElem xk x) * (FElem yk y) * (FElem out o') * R }.
-
-Require Import Curves.Edwards.XYZT.Precomputed. (* Move elsewhere *)
-
-Global Instance spec_of_add_precomputed : spec_of "add_precomputed" :=
-  fnspec! "add_precomputed"
-    (oxK oyK ozK otK X1K Y1K Z1K T1K ypx2K ymx2K xy2d2K : word) /
-    (ox oy oz ot X1 Y1 Z1 T1 ypx2 ymx2 xy2d2 : felem) (R : _ -> Prop),
-  { requires t m :=
-      bounded_by tight_bounds X1 /\
-      bounded_by tight_bounds Y1 /\
-      bounded_by tight_bounds Z1 /\ (* Could be loose if switch to mul *)
-      bounded_by loose_bounds T1 /\
-      bounded_by loose_bounds ypx2 /\
-      bounded_by loose_bounds ymx2 /\
-      bounded_by loose_bounds xy2d2 /\
-      m =* (FElem X1K X1) * (FElem Y1K Y1) * (FElem Z1K Z1) * (FElem T1K T1) * (FElem ypx2K ypx2) * (FElem ymx2K ymx2) * (FElem xy2d2K xy2d2) * (FElem oxK ox) * (FElem oyK oy) * (FElem ozK oz) * (FElem otK ot) * R;
-    ensures t' m' :=
-      t = t' /\
-      exists ox' oy' oz' ot',
-        (* Need to specify implicit parameters? *)
-        ((feval ox'), (feval oy'), (feval oz'), (feval ot')) = (@m1add_precomputed_coordinates (F M_pos) (F.add) (F.sub) (F.mul) ((feval X1), (feval Y1), (feval Z1), (feval T1)) ((feval ypx2), (feval ymx2), (feval xy2d2))) /\
-        bounded_by loose_bounds ox' /\
-        bounded_by loose_bounds oy' /\
-        bounded_by loose_bounds oz' /\
-        bounded_by loose_bounds ot' /\
-        m' =* (FElem X1K X1) * (FElem Y1K Y1) * (FElem Z1K Z1) * (FElem T1K T1) * (FElem ypx2K ypx2) * (FElem ymx2K ymx2) * (FElem xy2d2K xy2d2) * (FElem oxK ox') * (FElem oyK oy') * (FElem ozK oz') * (FElem otK ot') * R }.
-
-Local Instance spec_of_fe25519_square : spec_of "fe25519_square" := Field.spec_of_UnOp un_square.
-Local Instance spec_of_fe25519_mul : spec_of "fe25519_mul" := Field.spec_of_BinOp bin_mul.
-Local Instance spec_of_fe25519_add : spec_of "fe25519_add" := Field.spec_of_BinOp bin_add.
-Local Instance spec_of_fe25519_sub : spec_of "fe25519_sub" := Field.spec_of_BinOp bin_sub.
-
-Import WeakestPrecondition.
-
-From coqutil.Tactics Require Import Tactics letexists eabstract rdelta reference_to_string ident_of_string.
-Require Import bedrock2.Syntax.
-Require Import bedrock2.WeakestPrecondition.
-Require Import bedrock2.WeakestPreconditionProperties.
-Require Import bedrock2.Loops.
-Require Import bedrock2.Map.SeparationLogic bedrock2.Scalars.
+Local Instance spec_of_fe25519_from_word : spec_of "fe25519_from_word" := Field.spec_of_from_word.
+Local Instance spec_of_fe25519_from_bytes : spec_of "fe25519_from_bytes" := Field.spec_of_from_bytes.
+Local Instance spec_of_fe25519_to_bytes : spec_of "fe25519_to_bytes" := Field.spec_of_to_bytes.
+Local Instance spec_of_montladder : spec_of "montladder" := spec_of_montladder(Z.to_nat (Z.log2 Curve25519.order)).
 
 Local Arguments word.rep : simpl never.
 Local Arguments word.wrap : simpl never.
 Local Arguments word.unsigned : simpl never.
 Local Arguments word.of_Z : simpl never.
-Lemma square_and_add_ok : program_logic_goal_for_function! square_and_add.
+Lemma x25519_ok : program_logic_goal_for_function! x25519.
 Proof.
   repeat straightline.
-  repeat match goal with
-  | |- _ /\ _ => split
-  | |- call _ _ _ _ _ _ => straightline_call
-  | _ => straightline
-  end.
-  (* square *)
-  - (* square precondition bounds on x *) apply H1.
-  - (* mem sep for x *) eexists. ecancel_assumption.
-  - (* mem sep for out *) ecancel_assumption.
-  (* add *)
-  - (* add precondition bounds on x^2 *) apply H7.
-  - (* add precondition bounds on y *) apply H2.
-  - (* mem sep for o (holding x^2) *) eexists. ecancel_assumption.
-  - (* mem sep for y *) eexists. ecancel_assumption.
-  - (* mem sep for o (holding x^2+y) *) ecancel_assumption.
-  (* post-conditions *)
-  - exists x1. split. 2:split.
-    + (* math adds up *) simpl in H9. simpl in H6. rewrite H6 in H9. simpl. apply H9. (* Definitely better tactics for this *)
-    + (* postcondition bounds on out *) simpl in H10. simpl. apply H10. (* should just work to apply H10... *)
-    + (* postcondition mem sep *) ecancel_assumption.
+  seprewrite_in (@Bignum.Bignum_of_bytes _ _ _ _ _ _ 10 a) H2. { transitivity 40%nat; trivial. }
+
+  straightline_call; ssplit.
+  { eexists. ecancel_assumption. }
+  { cbv [Field.FElem].
+    use_sep_assumption. cancel. cancel_seps_at_indices 0%nat 0%nat; cbn; trivial. eapply RelationClasses.reflexivity. }
+  { unfold Field.bytes_in_bounds, frep25519, field_representation, Signature.field_representation, Representation.frep.
+    match goal with |- ?P ?x ?z => let y := eval cbv in x in change (P y z) end; cbn.
+    repeat (destruct p as [|? p]; try (cbn [length] in *;discriminate); []).
+    cbn; cbn [nth] in *.
+    cbv [COperationSpecifications.list_Z_bounded_by FoldBool.fold_andb_map map seq]; cbn.
+    pose proof byte.unsigned_range as HH. setoid_rewrite <-Le.Z.le_sub_1_iff in HH. cbn in HH.
+    setoid_rewrite Zle_is_le_bool in HH. setoid_rewrite <-Bool.andb_true_iff in HH.
+    rewrite 31HH; cbn.
+    eapply Bool.andb_true_iff; split; trivial.
+    eapply Bool.andb_true_iff; split; eapply Zle_is_le_bool; trivial.
+    eapply byte.unsigned_range. }
+  repeat straightline.
+
+  seprewrite_in (@Bignum.Bignum_of_bytes _ _ _ _ _ _ 10 a2) H15. { transitivity 40%nat; trivial. }
+
+  straightline_call; ssplit.
+  3: { unfold FElem, Field.FElem in *; extract_ex1_and_emp_in_goal; ssplit.
+       { use_sep_assumption. cancel; repeat ecancel_step.
+       cancel_seps_at_indices 0%nat 0%nat; trivial. cbn; reflexivity. }
+    all : eauto.
+    { instantiate (1:=None). exact I. } }
+  { reflexivity. }
+  { rewrite H3. vm_compute. inversion 1. }
+  repeat straightline.
+
+  cbv [FElem] in H22. extract_ex1_and_emp_in H22.
+  straightline_call; ssplit.
+  { ecancel_assumption. }
+  { transitivity 32%nat; auto. }
+  { eexists. ecancel_assumption. }
+  { intuition idtac. }
+  repeat straightline_cleanup.
+  repeat straightline.
+
+  cbv [Field.FElem] in *.
+  seprewrite_in @Bignum.Bignum_to_bytes H25.
+  seprewrite_in @Bignum.Bignum_to_bytes H25.
+  extract_ex1_and_emp_in H25.
+
+  repeat straightline; intuition eauto.
+  rewrite H29 in *. cbv [x25519_gallina].
+  use_sep_assumption; cancel. eapply RelationClasses.reflexivity.
 Qed.
 
-Local Ltac unwrap_calls :=
-  repeat match goal with
-  | |- _ /\ _ => split
-  | |- call _ _ _ _ _ _ => straightline_call
-  | _ => straightline
-  end.
+Global Instance spec_of_x25519_base : spec_of "x25519_base" :=
+  fnspec! "x25519_base" out sk / (o s : list Byte.byte) (R : _ -> Prop),
+  { requires t m := m =* s$@sk * o$@out * R /\
+      length s = 32%nat /\ length o = 32%nat;
+    ensures t' m := t=t' /\ m=* s$@sk ⋆ R ⋆
+      (le_split 32 (x25519_gallina (le_combine s) (F.of_Z _ 9)))$@out }.
 
-Local Ltac solve_bounds :=
-  repeat match goal with
-  | H: bounded_by loose_bounds _ |- bounded_by loose_bounds _ => apply H
-  | H: bounded_by tight_bounds _ |- bounded_by tight_bounds _ => apply H
-  | H: bounded_by _ _ |- bounded_by _ _ => cbv [un_xbounds bin_xbounds bin_ybounds un_square bin_mul bin_add un_outbounds bin_outbounds] in *
-  end.
-
-Local Ltac solve_mem :=
-  repeat match goal with
-  | |- exists _, _%sep _ => eexists
-  | |- _%sep _ => ecancel_assumption
-  end.
-
-Lemma square_and_add_ok2 : program_logic_goal_for_function! square_and_add.
+Lemma x25519_base_ok : program_logic_goal_for_function! x25519_base.
 Proof.
   repeat straightline.
-  unwrap_calls.
-  all: try solve_mem. all: try solve_bounds.
-  (* post-conditions *)
-  - exists x1. split. 2:split.
-    + (* math adds up *) simpl in H9. simpl in H6. rewrite H6 in H9. simpl. apply H9. (* Definitely better tactics for this *)
-    + (* postcondition bounds on out *) simpl in H10. simpl. apply H10. (* should just work to apply H10... *)
-    + (* postcondition mem sep *) ecancel_assumption.
-Qed.
-
-Lemma mul_and_add_ok : program_logic_goal_for_function! mul_and_add.
-Proof.
+  seprewrite_in (@Bignum.Bignum_of_bytes _ _ _ _ _ _ 10 a) H2. { transitivity 40%nat; trivial. }
+  straightline_call; ssplit.
+  { cbv [Field.FElem]. cbn. cbv [n]. ecancel_assumption. }
   repeat straightline.
-  repeat match goal with
-  | |- _ /\ _ => split
-  | |- call _ _ _ _ _ _ => straightline_call
-  | _ => straightline
-  end.
-  (* square *)
-  - (* mul precondition bounds on x *) apply H1.
-  - (* same bounds gain *) apply H1.
-  - (* mem sep for x *) eexists. ecancel_assumption.
-  - (* same mem sep again *) eexists. ecancel_assumption.
-  - (* mem sep for out *) ecancel_assumption.
-  (* add *)
-  - (* add precondition bounds on x^2 *) apply H7.
-  - (* add precondition bounds on y *) apply H2.
-  - (* mem sep for o (holding x^2) *) eexists. ecancel_assumption.
-  - (* mem sep for y *) eexists. ecancel_assumption.
-  - (* mem sep for o (holding x^2+y) *) ecancel_assumption.
-  (* post-conditions *)
-  - exists x1. split. 2:split.
-    + (* math adds up *) simpl in H9. simpl in H6. rewrite H6 in H9. simpl. apply H9. (* Definitely better tactics for this *)
-    + (* postcondition bounds on out *) simpl in H10. simpl. apply H10. (* should just work to apply H10... *)
-    + (* postcondition mem sep *) ecancel_assumption.
+
+  seprewrite_in (@Bignum.Bignum_of_bytes _ _ _ _ _ _ 10 a2) H13. { transitivity 40%nat; trivial. }
+
+  straightline_call; ssplit.
+  3: { unfold FElem, Field.FElem in *; extract_ex1_and_emp_in_goal; ssplit.
+       { use_sep_assumption. cancel; repeat ecancel_step.
+       cancel_seps_at_indices 0%nat 0%nat; trivial. cbn; reflexivity. }
+    all : eauto.
+    { instantiate (1:=None). exact I. } }
+  { reflexivity. }
+  { rewrite H3. vm_compute. inversion 1. }
+  repeat straightline.
+
+  unfold FElem in H20. extract_ex1_and_emp_in H20.
+  straightline_call; ssplit.
+  { ecancel_assumption. }
+  { transitivity 32%nat; auto. }
+  { eexists. ecancel_assumption. }
+  { intuition idtac. }
+  repeat straightline_cleanup.
+  repeat straightline.
+
+  cbv [Field.FElem] in *.
+  seprewrite_in @Bignum.Bignum_to_bytes H23.
+  seprewrite_in @Bignum.Bignum_to_bytes H23.
+  extract_ex1_and_emp_in H23.
+
+  repeat straightline; intuition eauto.
+  rewrite H27 in *. cbv [x25519_gallina].
+  use_sep_assumption; cancel. eapply RelationClasses.reflexivity.
 Qed.
 
+Require Import coqutil.Word.Naive.
+Require Import coqutil.Macros.WithBaseName.
+
+Definition felem_cswap := CSwap.felem_cswap(word:=word32)(field_parameters:=field_parameters)(field_representaton:=field_representation n s c).
+Definition fe25519_inv := fe25519_inv(word:=word32)(field_parameters:=field_parameters).
+
+Definition funcs :=
+  &[,x25519; x25519_base;
+    montladder;
+    fe25519_to_bytes;
+    fe25519_from_bytes;
+    fe25519_from_word;
+    felem_cswap;
+    fe25519_copy;
+    fe25519_inv;
+    ladderstep;
+    fe25519_mul;
+    fe25519_add;
+    fe25519_sub;
+    fe25519_square;
+    fe25519_scmula24 ].
+
+Require Import bedrock2.ToCString.
+Definition montladder_c_module := list_byte_of_string (ToCString.c_module funcs).
+
+#[export]
+Instance BWM_RV32IM : FlatToRiscvCommon.bitwidth_iset 32 Decode.RV32IM := eq_refl.
+
+Derive montladder_compiler_result SuchThat
+       (compile
+         (compile_ext_call (funname_env:=SortedListString.map))
+         funcs = Success montladder_compiler_result)
+       As montladder_compiler_result_ok.
+Proof.
+  match goal with x := _ |- _ => cbv delta [x]; clear x end.
+  match goal with |- ?a = _ => set a end.
+  vm_compute.
+  match goal with |- @Success ?A ?x = Success ?e => is_evar e;
+    exact (@eq_refl (result A) (@Success A x)) end.
+Qed.
+
+Definition montladder_stack_size := snd montladder_compiler_result.
+Definition montladder_finfo := snd (fst montladder_compiler_result).
+Definition montladder_insns := fst (fst montladder_compiler_result).
+Definition montladder_bytes := Pipeline.instrencode montladder_insns.
+Definition montladder_symbols : list byte := Symbols.symbols montladder_finfo.
+
+
+Require riscv.Utility.InstructionNotations.
+Require riscv.Utility.InstructionCoercions.
+Module PrintAssembly.
+  Import riscv.Utility.InstructionNotations.
+  Import riscv.Utility.InstructionCoercions.
+  Unset Printing Coercions.
+
+  (* Compute garagedoor_finfo. (* fe25519_mul is more than 10KB in just one function *) *)
+  Goal True. let r := eval cbv in montladder_insns in idtac (* r *). Abort.
+End PrintAssembly.
